Module-based reorganization of Qhasm code

src/Assembly/Qhasm.v
@@ -1,674 +1,73 @@
+Require Import QhasmEvalCommon.
+Require Import Language.
+Require Import List NPeano.
 
-Require Import String List.
-Require Import Bedrock.Word.
-Require Import ZArith NArith NPeano.
-Require Import Coq.Structures.OrderedTypeEx.
+Module Qhasm <: Language.
+  Import ListNotations.
 
-Require Export FMapAVL FMapList.
+  (* A constant upper-bound on the number of operations we run *)
+  Definition maxOps: nat := 1000.
+  Definition State := State.
 
-Module NatM := FMapAVL.Make(Nat_as_OT).
-Definition DefMap: Type := NatM.t N.
-Definition StateMap: Type := NatM.t DefMap.
-Definition LabelMap: Type := NatM.t nat.
+  (* Program Types *)
+  Inductive QhasmStatement :=
+    | QAssign: Assignment -> QhasmStatement
+    | QOp: Operation -> QhasmStatement
+    | QJmp: Conditional -> Label -> QhasmStatement
+    | QLabel: Label -> QhasmStatement.
 
-(* A formalization of x86 qhasm *)
+  Hint Constructors QhasmStatement.
 
-(* Basic Types *)
-Definition Label := nat.
-Definition Index (limit: nat) := {x: nat | (x < limit)%nat}.
-Definition Invert := bool.
+  Definition Program := list QhasmStatement.
 
-Definition indexToNat {lim: nat} (i: Index lim): nat := proj1_sig i.
-Coercion indexToNat : Index >-> nat.
+  (* Only execute while loops a fixed number of times.
+     TODO (rsloan): can we do any better? *)
 
-(* A constant upper-bound on the number of operations we run *)
-Definition maxOps: nat := 1000.
-
-(* Datatypes *)
-Inductive Const: nat -> Set :=
-  | const32: word 32 -> Const 32
-  | const64: word 64 -> Const 64
-  | const128: word 128 -> Const 128.
-
-Inductive Reg: nat -> Set :=
-  | reg32: nat -> Reg 32
-  | reg3232: nat -> Reg 64
-  | reg6464: nat -> Reg 128
-  | reg80: nat -> Reg 80.
-
-Inductive Stack: nat -> Set :=
-  | stack32: nat -> Stack 32
-  | stack64: nat -> Stack 64
-  | stack128: nat -> Stack 128.
-
-(* Assignments *)
-Inductive Assignment : Set :=
-  | Assign32Stack32: Reg 32 -> Stack 32 -> Assignment
-  | Assign32Stack16: Reg 32 -> Stack 32 -> Index 2 -> Assignment
-  | Assign32Stack8: Reg 32 -> Stack 32 -> Index 4 -> Assignment
-  | Assign32Stack64: Reg 32 -> Stack 64 -> Index 2 -> Assignment
-  | Assign32Stack128: Reg 32 -> Stack 128 -> Index 2 -> Assignment
-
-  | Assign32Reg32: Reg 32 -> Reg 32 -> Assignment
-  | Assign32Reg16: Reg 32 -> Reg 32 -> Index 2 -> Assignment
-  | Assign32Reg8: Reg 32 -> Reg 32 -> Index 4 -> Assignment
-  | Assign32Reg64: Reg 32 -> Reg 64 -> Index 2 -> Assignment
-  | Assign32Reg128: Reg 32 -> Reg 128 -> Index 4 -> Assignment
-
-  | Assign3232Stack32: Reg 64 -> Index 2 -> Stack 32 -> Assignment
-  | Assign3232Stack64: Reg 64 -> Stack 64 -> Assignment
-  | Assign3232Stack128: Reg 64 -> Stack 128 -> Index 2 -> Assignment
-
-  | Assign3232Reg32: Reg 64 -> Index 2 -> Reg 32 -> Assignment
-  | Assign3232Reg64: Reg 64 -> Reg 64 -> Assignment
-  | Assign3232Reg128: Reg 64 -> Reg 128 -> Index 2 -> Assignment
-
-  | Assign6464Reg32: Reg 128 -> Index 4 -> Reg 32 -> Assignment
-  | Assign6464Reg64: Reg 128 -> Index 2 -> Reg 64 -> Assignment
-  | Assign6464Reg128: Reg 128 -> Reg 128 -> Assignment
-
-  | AssignConstant: Reg 32 -> Const 32 -> Assignment.
-
-Hint Constructors Assignment.
-
-(* Operations *)
-
-Inductive BinOp :=
-  | Plus: BinOp | Minus: BinOp | Mult: BinOp
-  | Div: BinOp | Xor: BinOp | And: BinOp | Or: BinOp.
-
-Inductive RotOp :=
-  | Shl: RotOp | Shr: RotOp | Rotl: RotOp | Rotr: RotOp.
-
-Inductive Operation :=
-  | OpReg32Constant: BinOp -> Reg 32 -> Const 32 -> Operation
-  | OpReg32Reg32: BinOp -> Reg 32 -> Reg 32 -> Operation
-  | RotReg32: RotOp -> Reg 32 -> Index 32 -> Operation
-
-  | OpReg64Constant: BinOp -> Reg 64 -> Const 64 -> Operation
-  | OpReg64Reg64: BinOp -> Reg 64 -> Reg 64 -> Operation
-
-  | OpReg128Constant: BinOp -> Reg 128 -> Const 32 -> Operation
-  | OpReg128Reg128: BinOp -> Reg 128 -> Reg 128 -> Operation.
-
-Hint Constructors Operation.
-
-(* Control Flow *)
-
-Inductive TestOp :=
-  | TEq: TestOp
-  | TLt: TestOp
-  | TUnsignedLt: TestOp
-  | TGt: TestOp
-  | TUnsignedGt: TestOp.
-
-Inductive Conditional :=
-  | TestTrue: Conditional
-  | TestFalse: Conditional
-  | TestReg32Reg32: TestOp -> Invert -> Reg 32 -> Reg 32 -> Conditional
-  | TestReg32Const: TestOp -> Invert -> Reg 32 -> Const 32 -> Conditional.
-
-Definition invertConditional (c: Conditional): Conditional :=
-  match c with
-  | TestTrue => TestFalse
-  | TestFalse => TestFalse
-  | TestReg32Reg32 o i r0 r1 => TestReg32Reg32 o (negb i) r0 r1
-  | TestReg32Const o i r c => TestReg32Const o (negb i) r c
-  end.
-
-Hint Constructors Conditional.
-
-(* Program Types *)
-
-Inductive AlmostQhasm :=
-  | ASeq: AlmostQhasm -> AlmostQhasm -> AlmostQhasm
-  | AAssign: Assignment -> AlmostQhasm
-  | AOp: Operation -> AlmostQhasm 
-  | ACond: Conditional -> AlmostQhasm -> AlmostQhasm
-  | AWhile: Conditional -> AlmostQhasm -> AlmostQhasm.
-
-Hint Constructors AlmostQhasm.
-
-Inductive QhasmStatement :=
-  | QAssign: Assignment -> QhasmStatement
-  | QOp: Operation -> QhasmStatement
-  | QJmp: Conditional -> Label -> QhasmStatement
-  | QLabel: Label -> QhasmStatement.
-
-Hint Constructors QhasmStatement.
-
-Definition Qhasm := list QhasmStatement.
-
-Import ListNotations.
-
-(* AlmostQhasm -> Qhasm Conversion *)
-
-Fixpoint almostToQhasm' (prog: AlmostQhasm) (startLabel: N): Qhasm :=
-  let label0 := N.shiftl 1 startLabel in
-  let label1 := N.succ label0 in
-
-  match prog with
-  | ASeq a b => (almostToQhasm' a label0) ++ (almostToQhasm' b label1)
-  | AAssign a => [ QAssign a ]
-  | AOp a => [ QOp a ]
-  | ACond c a =>
-    [QJmp (invertConditional c) (N.to_nat label0)] ++
-    (almostToQhasm' a label1) ++
-    [QLabel (N.to_nat label0)]
-  | AWhile c a =>
-    let start := N.to_nat (N.shiftl 1 label0) in
-    let finish := S start in
-    [ QJmp (invertConditional c) finish ;
-      QLabel start ] ++
-      (almostToQhasm' a label1) ++
-    [ QJmp c start;
-      QLabel finish ]
-  end.
-
-Definition almostToQhasm (prog: AlmostQhasm) := almostToQhasm' prog 0%N.
-
-(* Machine State *)
-
-Inductive State :=
-| fullState (regState: StateMap) (stackState: StateMap): State.
-
-Definition getReg {n} (reg: Reg n) (state: State): option (word n).
-  destruct state; inversion reg as [L H | L H | L H | L H];
-    destruct (NatM.find n regState) as [map |];
-    first [ destruct (NatM.find L map) as [n0 |] | exact None ];
-    first [ rewrite H; exact (Some (NToWord n n0)) | exact None ].
-Defined.
-
-Definition setReg {n} (reg: Reg n) (value: word n) (state: State): State.
-  inversion state; inversion reg as [L H | L H | L H | L H];
-    destruct (NatM.find n regState) as [map |];
-    first [
-       exact
-         (fullState
-           (NatM.add n
-             (NatM.add L (wordToN value) map) regState)
-             stackState)
-     | exact state ].
-Defined.
-
-Definition getStack {n} (entry: Stack n) (state: State): option (word n).
-  destruct state; inversion entry as [L H | L H | L H];
-    destruct (NatM.find n stackState) as [map |];
-    first [ destruct (NatM.find L map) as [n0 |] | exact None ];
-    first [ rewrite H; exact (Some (NToWord n n0)) | exact None ].
-Defined.
-
-Definition setStack {n} (entry: Stack n) (value: word n) (state: State): State.
-  inversion state; inversion entry as [L H | L H | L H];
-    destruct (NatM.find n stackState) as [map |];
-    first [
-       exact
-         (fullState regState
-           (NatM.add n
-             (NatM.add L (wordToN value) map) regState))
-     | exact state ].
-Defined.
-
-Definition emptyState: State :=
-  fullState (NatM.empty DefMap) (NatM.empty DefMap).
-
-(* Magical Bitwise Manipulations *)
-
-(* Force w to be m bits long, by truncation or zero-extension *)
-Definition trunc {n} (m: nat) (w: word n): word m.
-  destruct (lt_eq_lt_dec n m) as [s|s]; try destruct s as [s|s].
-
-  - replace m with (n + (m - n)) by abstract intuition.
-    refine (zext w (m - n)).
-
-  - rewrite <- s; assumption.
-
-  - replace n with (m + (n - m)) in w by abstract intuition.
-    refine (split1 m (n-m) w).
-Defined.
-
-(* Get the index-th m-bit block of w *)
-Definition getIndex {n} (w: word n) (m index: nat): word m.
-  replace n with
-    ((min n (m * index)) + (n - (min n (m * index))))%nat
-    in w by abstract (
-      assert ((min n (m * index)) <= n)%nat
-        by apply Nat.le_min_l;
-      intuition).
-
-  refine
-    (trunc m
-      (split2 (min n (m * index)) (n - min n (m * index)) w)).
-Defined.
-
-(* set the index-th m-bit block of w to s *)
-Definition setInPlace {n m} (w: word n) (s: word m) (index: nat): word n :=
-  w ^& (wnot (trunc n (combine (wones m) (wzero (index * m)%nat))))
-    ^| (trunc n (combine s (wzero (index * m)%nat))).
-
-(* State Evaluation *)
-
-Definition evalTest {n} (o: TestOp) (invert: bool) (a b: word n): bool :=
-  xorb invert
-  match o with
-  | TEq => weqb a b
-  | TLt =>
-    match (Z.compare (wordToZ a) (wordToZ b)) with
-    | Lt => true
-    | _ => false
-    end
-  | TUnsignedLt =>
-    match (N.compare (wordToN a) (wordToN b)) with
-    | Lt => true
-    | _ => false
-    end
-  | TGt =>
-    match (Z.compare (wordToZ a) (wordToZ b)) with
-    | Gt => true
-    | _ => false
-    end
-  | TUnsignedGt =>
-    match (N.compare (wordToN a) (wordToN b)) with
-    | Gt => true
-    | _ => false
-    end
-  end.
-
-
-Definition evalCond (c: Conditional) (state: State): option bool :=
-  match c with
-  | TestTrue => Some true
-  | TestFalse => Some false
-  | TestReg32Reg32 o i r0 r1 =>
-    match (getReg r0 state) with
-    | Some v0 =>
-      match (getReg r0 state) with
-      | Some v1 => Some (evalTest o i v0 v1)
-      | _ => None
+  Fixpoint getLabelMap' (prog: Program) (cur: LabelMap) (index: nat): LabelMap :=
+    match prog with
+    | p :: ps =>
+      match p with
+      | QLabel label => getLabelMap' ps (NatM.add label index cur) (S index)
+      | _ => getLabelMap' ps cur (S index)
       end
-    | _ => None
-    end
-  | TestReg32Const o i r x =>
-    match (getReg r state) with
-    | Some v0 =>
-      match x with
-      | const32 v1 => Some (evalTest o i v0 v1)
+    | [] => cur
+    end.
+
+  Definition getLabelMap (prog: Program): LabelMap :=
+    getLabelMap' prog (NatM.empty nat) O.
+
+  Fixpoint eval' (prog: Program) (state: State) (loc: nat) (horizon: nat) (labelMap: LabelMap) (maxLoc: nat): option State :=
+    match horizon with
+    | (S h) =>
+      match (nth_error prog loc) with
+      | Some stmt =>
+        let (nextState, jmp) :=
+          match stmt with
+          | QAssign a => (evalAssignment a state, None)
+          | QOp o => (evalOperation o state, None)
+          | QLabel l => (state, None)
+          | QJmp c l =>
+            if (evalCond c state)
+            then (state, Some l)
+            else (state, None)
+          end
+        in
+          match jmp with
+          | None =>
+            if (Nat.eq_dec loc maxLoc)
+            then Some nextState
+            else eval' prog nextState (S loc) h labelMap maxLoc
+          | Some nextLoc =>
+            eval' prog nextState nextLoc h labelMap nextLoc
+          end
+      | None => None
       end
-    | _ => None
-    end
-  end.
+    | O => None
+    end.
 
-Definition evalBinOp {n} (o: BinOp) (a b: word n): word n :=
-  match o with
-  | Plus => wplus a b
-  | Minus => wminus a b
-  | Mult => wmult a b
-  | Div => NToWord n ((wordToN a) / (wordToN b))%N
-  | Or => wor a b
-  | Xor => wxor a b
-  | And => wand a b
-  end.
+  Definition eval (prog: Program) (state: State): option State :=
+    eval' prog state O maxOps (getLabelMap prog) ((length prog) - 1).
 
-Definition evalRotOp {n} (o: RotOp) (a: word n) (m: nat): word n :=
-  match o with
-  | Shl => NToWord n (N.shiftl_nat (wordToN a) m)
-  | Shr => NToWord n (N.shiftr_nat (wordToN a) m)
+  (* world peace *)
+End Qhasm.
 
-  (* TODO (rsloan): not actually rotate operations *)
-  | Rotl => NToWord n (N.shiftl_nat (wordToN a) m) 
-  | Rotr => NToWord n (N.shiftr_nat (wordToN a) m)
-  end.
-
-Definition evalOperation (o: Operation) (state: State): State :=
-  match o with
-  | OpReg32Constant b r c =>
-    match (getReg r state) with
-    | Some v0 =>
-      match c with
-      | const32 v1 => setReg r (evalBinOp b v0 v1) state
-      | _ => state
-      end
-    | None => state
-    end
-  | OpReg32Reg32 b r0 r1 =>
-    match (getReg r0 state) with
-    | Some v0 =>
-      match (getReg r1 state) with
-      | Some v1 => setReg r0 (evalBinOp b v0 v1) state
-      | _ => state
-      end
-    | None => state
-    end
-  | RotReg32 b r m =>
-    match (getReg r state) with
-    | Some v0 => setReg r (evalRotOp b v0 m) state
-    | None => state
-    end
-
-  | OpReg64Constant b r c =>
-    match (getReg r state) with
-    | Some v0 =>
-      match c with
-      | const64 v1 => setReg r (evalBinOp b v0 v1) state
-      | _ => state
-      end
-    | None => state
-    end
-  | OpReg64Reg64 b r0 r1 =>
-    match (getReg r0 state) with
-    | Some v0 =>
-      match (getReg r1 state) with
-      | Some v1 => setReg r0 (evalBinOp b v0 v1) state
-      | _ => state
-      end
-    | None => state
-    end
-
-  | OpReg128Constant b r c =>
-    match (getReg r state) with
-    | Some v0 =>
-      match c with
-      | const128 v1 => setReg r (evalBinOp b v0 v1) state
-      | _ => state
-      end
-    | None => state
-    end
-  | OpReg128Reg128 b r0 r1 => 
-    match (getReg r0 state) with
-    | Some v0 =>
-      match (getReg r1 state) with
-      | Some v1 => setReg r0 (evalBinOp b v0 v1) state
-      | _ => state
-      end
-    | None => state
-    end
-  end.
-
-Definition evalAssignment (a: Assignment) (state: State): State :=
-  match a with
-  | Assign32Stack32 r s =>
-    match (getReg r state) with
-    | Some v0 =>
-      match (getStack s state) with
-      | Some v1 => setReg r v1 state
-      | _ => state
-      end
-    | None => state
-    end
-  | Assign32Stack16 r s i =>
-    match (getReg r state) with
-    | Some v0 =>
-      match (getStack s state) with
-      | Some v1 => setReg r (trunc 32 (getIndex v1 16 i)) state
-      | _ => state
-      end
-    | None => state
-    end
-  | Assign32Stack8 r s i =>
-    match (getReg r state) with
-    | Some v0 =>
-      match (getStack s state) with
-      | Some v1 => setReg r (trunc 32 (getIndex v1 8 i)) state
-      | _ => state
-      end
-    | None => state
-    end
-  | Assign32Stack64 r s i =>
-    match (getReg r state) with
-    | Some v0 =>
-      match (getStack s state) with
-      | Some v1 => setReg r (getIndex v1 32 i) state
-      | _ => state
-      end
-    | None => state
-    end
-  | Assign32Stack128 r s i =>
-    match (getReg r state) with
-    | Some v0 =>
-      match (getStack s state) with
-      | Some v1 => setReg r (getIndex v1 32 i) state
-      | _ => state
-      end
-    | None => state
-    end
-
-  | Assign32Reg32 r0 r1 =>
-    match (getReg r0 state) with
-    | Some v0 =>
-      match (getReg r1 state) with
-      | Some v1 => setReg r0 v1 state
-      | _ => state
-      end
-    | None => state
-    end
-  | Assign32Reg16 r0 r1 i =>
-    match (getReg r0 state) with
-    | Some v0 =>
-      match (getReg r1 state) with
-      | Some v1 => setReg r0 (trunc 32 (getIndex v1 16 i)) state
-      | _ => state
-      end
-    | None => state
-    end
-  | Assign32Reg8 r0 r1 i =>
-    match (getReg r0 state) with
-    | Some v0 =>
-      match (getReg r1 state) with
-      | Some v1 => setReg r0 (trunc 32 (getIndex v1 8 i)) state
-      | _ => state
-      end
-    | None => state
-    end
-  | Assign32Reg64 r0 r1 i =>
-    match (getReg r0 state) with
-    | Some v0 =>
-      match (getReg r1 state) with
-      | Some v1 => setReg r0 (getIndex v1 32 i) state
-      | _ => state
-      end
-    | None => state
-    end
-  | Assign32Reg128 r0 r1 i =>
-    match (getReg r0 state) with
-    | Some v0 =>
-      match (getReg r1 state) with
-      | Some v1 => setReg r0 (getIndex v1 32 i) state
-      | _ => state
-      end
-    | None => state
-    end
-
-  | Assign3232Stack32 r0 i s =>
-    match (getReg r0 state) with
-    | Some v0 =>
-      match (getStack s state) with
-      | Some v1 => setReg r0 (setInPlace v0 v1 i) state
-      | _ => state
-      end
-    | None => state
-    end
-
-  | Assign3232Stack64 r s =>
-    match (getReg r state) with
-    | Some v0 =>
-      match (getStack s state) with
-      | Some v1 => setReg r v1 state
-      | _ => state
-      end
-    | None => state
-    end
-
-  | Assign3232Stack128 r s i =>
-    match (getReg r state) with
-    | Some v0 =>
-      match (getStack s state) with
-      | Some v1 => setReg r (getIndex v1 64 i) state
-      | _ => state
-      end
-    | None => state
-    end
-
-  | Assign3232Reg32 r0 i r1 =>
-    match (getReg r0 state) with
-    | Some v0 =>
-      match (getReg r1 state) with
-      | Some v1 => setReg r0 (setInPlace v0 v1 i) state
-      | _ => state
-      end
-    | None => state
-    end
-
-  | Assign3232Reg64 r0 r1 =>
-    match (getReg r0 state) with
-    | Some v0 =>
-      match (getReg r1 state) with
-      | Some v1 => setReg r0 v1 state
-      | _ => state
-      end
-    | None => state
-    end
-
-  | Assign3232Reg128 r0 r1 i =>
-    match (getReg r0 state) with
-    | Some v0 =>
-      match (getReg r1 state) with
-      | Some v1 => setReg r0 (getIndex v1 64 i) state
-      | _ => state
-      end
-    | None => state
-    end
-
-  | Assign6464Reg32 r0 i r1 =>
-    match (getReg r0 state) with
-    | Some v0 =>
-      match (getReg r1 state) with
-      | Some v1 => setReg r0 (setInPlace v0 v1 i) state
-      | _ => state
-      end
-    | None => state
-    end
-
-  | Assign6464Reg64 r0 i r1 =>
-    match (getReg r0 state) with
-    | Some v0 =>
-      match (getReg r1 state) with
-      | Some v1 => setReg r0 (setInPlace v0 v1 i) state
-      | _ => state
-      end
-    | None => state
-    end
-
-  | Assign6464Reg128 r0 r1 =>
-    match (getReg r0 state) with
-    | Some v0 =>
-      match (getReg r1 state) with
-      | Some v1 => setReg r0 v1 state
-      | _ => state
-      end
-    | None => state
-    end
-
-  | AssignConstant r c =>
-    match (getReg r state) with
-    | Some v0 =>
-      match c with
-      | const32 v1 => setReg r v1 state
-      | _ => state
-      end
-    | None => state
-    end
-  end.
-
-(* AlmostQhasm Evaluation *)
-
-
-(* Only execute while loops a fixed number of times.
-   TODO (rsloan): can we do any better? *)
-
-Fixpoint almostEvalWhile (cond: Conditional) (prog: AlmostQhasm) (state: State) (horizon: nat): State :=
-  match horizon with
-  | (S m) => 
-    if (evalCond cond state)
-    then almostEvalWhile cond prog state m
-    else state 
-  | O => state
-  end.
-
-Fixpoint almostEval (prog: AlmostQhasm) (state: State): State :=
-  match prog with
-  | ASeq a b => almostEval b (almostEval a state)
-  | AAssign a => evalAssignment a state
-  | AOp a => evalOperation a state
-  | ACond c a =>
-    if (evalCond c state)
-    then almostEval a state
-    else state 
-  | AWhile c a => almostEvalWhile c a state maxOps
-  end.
-
-Definition almostEvalReg {n} (prog: AlmostQhasm) (reg: Reg n): option (word n) :=
-  getReg reg (almostEval prog emptyState).
-
-Definition almostEvalStack {n} (prog: AlmostQhasm) (stack: Stack n): option (word n) :=
-  getStack stack (almostEval prog emptyState).
-
-(* Qhasm Evaluation *)
-
-Fixpoint getLabelMap' (prog: Qhasm) (cur: LabelMap) (index: nat): LabelMap :=
-  match prog with
-  | p :: ps =>
-    match p with
-    | QLabel label => getLabelMap' ps (NatM.add label index cur) (S index)
-    | _ => getLabelMap' ps cur (S index)
-    end
-  | [] => cur
-  end.
-
-Definition getLabelMap (prog: Qhasm): LabelMap :=
-  getLabelMap' prog (NatM.empty nat) O.
-
-Fixpoint eval' (prog: Qhasm) (state: State) (loc: nat) (horizon: nat) (labelMap: LabelMap) (maxLoc: nat): option State :=
-  match horizon with
-  | (S h) =>
-    match (nth_error prog loc) with
-    | Some stmt =>
-      let (nextState, jmp) :=
-        match stmt with
-        | QAssign a => (evalAssignment a state, None)
-        | QOp o => (evalOperation o state, None)
-        | QLabel l => (state, None)
-        | QJmp c l =>
-          if (evalCond c state)
-          then (state, Some l)
-          else (state, None)
-        end
-      in
-        match jmp with
-        | None =>
-          if (Nat.eq_dec loc maxLoc)
-          then Some nextState
-          else eval' prog nextState (S loc) h labelMap maxLoc
-        | Some nextLoc =>
-          eval' prog nextState nextLoc h labelMap nextLoc
-        end
-    | None => None
-    end
-  | O => None
-  end.
-
-Definition eval (prog: Qhasm) (state: State): option State :=
-  eval' prog state O maxOps (getLabelMap prog) ((length prog) - 1).
-
-Definition evalReg {n} (prog: Qhasm) (reg: Reg n): option (word n) :=
-  match (eval prog emptyState) with
-  | Some st => getReg reg st
-  | None => None
-  end.
-
-Definition evalStack {n} (prog: Qhasm) (stack: Stack n): option (word n) :=
-  match (eval prog emptyState) with
-  | Some st => getStack stack st
-  | None => None
-  end.
-
-(* world peace *)
