src/Assembly/AlmostQhasm.v
@@ -1,0 +1,57 @@
+Require Import QhasmEvalCommon.
+Require Import Language.
+Require Import List.
+
+Module AlmostQhasm <: Language.
+  Import ListNotations.
+
+  (* A constant upper-bound on the number of operations we run *)
+  Definition maxOps: nat := 1000.
+
+  (* Program Types *)
+  Definition State := State.
+
+  Inductive AlmostProgram: Set :=
+    | ASkip: AlmostProgram
+    | ASeq: AlmostProgram -> AlmostProgram -> AlmostProgram
+    | AAssign: Assignment -> AlmostProgram
+    | AOp: Operation -> AlmostProgram
+    | ACond: Conditional -> AlmostProgram -> AlmostProgram -> AlmostProgram
+    | AWhile: Conditional -> AlmostProgram -> AlmostProgram.
+
+  Hint Constructors AlmostProgram.
+
+  Definition Program := AlmostProgram.
+
+  (* Only execute while loops a fixed number of times.
+     TODO (rsloan): can we do any better? *)
+
+  (* TODO: make this inductive *)
+  Fixpoint almostEvalWhile (cond: Conditional) (prog: Program) (state: State) (horizon: nat): option State :=
+    match horizon with
+    | (S m) =>
+      if (evalCond cond state)
+      then almostEvalWhile cond prog state m
+      else Some state
+    | O => None
+    end.
+
+  Fixpoint eval (prog: Program) (state: State): option State :=
+    match prog with
+    | ASkip => Some state
+    | ASeq a b =>
+      match (eval a state) with
+      | (Some st') => eval b st'
+      | _ => None
+      end
+    | AAssign a => Some (evalAssignment a state)
+    | AOp a => Some (evalOperation a state)
+    | ACond c a b =>
+      if (evalCond c state)
+      then eval a state
+      else eval b state
+    | AWhile c a => almostEvalWhile c a state maxOps
+    end.
+
+  (* world peace *)
+End AlmostQhasm.
