src/Assembly/Conversion.v
@@ -1,0 +1,19 @@
+
+Require Export Language.
+
+Module Type Conversion (A B: Language).
+
+  Parameter convertProgram: A.Program -> option B.Program.
+  Parameter convertState: B.State -> option A.State.
+
+  Axiom convert_spec: forall st' prog,
+    match ((convertProgram prog), (convertState st')) with
+    | (Some prog', Some st) =>
+      match (B.eval prog' st') with
+      | Some st'' => A.eval prog st = (convertState st'')
+      | _ => True
+      end
+    | _ => True
+    end.
+
+End Conversion.
