src/Assembly/HighLevel.v
@@ -1,9 +1,0 @@
-
-Inductive Const32 : Set = | const32: word 32 -> Const32.
-
-Inductive HL :=
-  | Input: Const32 -> HL
-  | Variable: Const32 -> HL
-  | Let: forall m, nat -> HL -> HL -> HL
-  | Lift1: (Const32 -> Const32) -> HL -> HL
-  | Lift2: (Const32 -> Const32 -> Const32) -> HL -> HL -> HL.
