src/Assembly/StringConversion.v
@@ -1,0 +1,30 @@
+Require Export Qhasm Language Conversion.
+Require Export String.
+
+Module QhasmString <: Language.
+  Definition Program := string.
+  Definition State := unit.
+
+  Definition eval (p: Program) (s: State): option State := Some tt.
+End QhasmString.
+
+Module StringConversion <: Conversion Qhasm QhasmString.
+
+  Definition convertState (st: QhasmString.State): option Qhasm.State := None.
+
+  (* TODO (rsloan): Actually implement string conversion *)
+  Definition convertProgram (prog: Qhasm.Program): option string :=
+    Some EmptyString.
+
+  Lemma convert_spec: forall st' prog,
+    match ((convertProgram prog), (convertState st')) with
+    | (Some prog', Some st) =>
+      match (QhasmString.eval prog' st') with
+      | Some st'' => Qhasm.eval prog st = (convertState st'')
+      | _ => True
+      end
+    | _ => True
+    end.
+  Admitted.
+
+End StringConversion.
